Prefix(:=<http://usefulinc.com/ns/doap#>)
Prefix(dc:=<http://purl.org/dc/elements/1.1/>)
Prefix(vs:=<http://www.w3.org/2003/06/sw-vocab-status/ns#>)
Prefix(owl:=<http://www.w3.org/2002/07/owl#>)
Prefix(rdf:=<http://www.w3.org/1999/02/22-rdf-syntax-ns#>)
Prefix(xml:=<http://www.w3.org/XML/1998/namespace>)
Prefix(xsd:=<http://www.w3.org/2001/XMLSchema#>)
Prefix(doap:=<http://usefulinc.com/ns/doap#>)
Prefix(foaf:=<http://xmlns.com/foaf/0.1/>)
Prefix(rdfs:=<http://www.w3.org/2000/01/rdf-schema#>)


Ontology(<http://usefulinc.com/ns/doap#>
Import(<http://xmlns.com/foaf/0.1/index.rdf>)
Annotation(dc:creator "Edd Wilder-James")
Annotation(dc:description "Das Vokabular \"Description of a Project (DOAP)\", beschrieben durch W3C RDF Schema and the Web Ontology Language."@de)
Annotation(dc:description "El vocabulario Description of a Project (DOAP, Descripción de un Proyecto), descrito usando RDF Schema de W3C
		y Web Ontology Language."@es)
Annotation(dc:description "Le vocabulaire Description Of A Project (DOAP, Description D'Un Projet),
		décrit en utilisant RDF Schema du W3C et OWL."@fr)
Annotation(dc:description "Slovník Description of a Project (DOAP, Popis projektu), popsaný použitím W3C RDF Schema a Web Ontology Language."@cs)
Annotation(dc:description "The Description of a Project (DOAP) vocabulary, described using W3C RDF Schema and the Web Ontology Language.")
Annotation(dc:description "Vocabulário de descrição de um Projeto (DOAP - Description of a Project), descrito no esquema (schema) W3C RDF e na Web Ontology Language."@pt)
Annotation(dc:format "application/rdf+xml")
Annotation(dc:rights "Copyright © The DOAP Authors")
Annotation(dc:title "Description of a Project (DOAP) vocabulary")

Declaration(Class(<http://rdfs.org/sioc/ns#Container>))
Declaration(Class(<http://rdfs.org/sioc/types#MailingList>))
Declaration(Class(<http://rdfs.org/sioc/types#Weblog>))
Declaration(Class(<http://rdfs.org/sioc/types#Wiki>))
Declaration(Class(doap:ArchRepository))
Declaration(Class(doap:BKRepository))
Declaration(Class(doap:BazaarBranch))
Declaration(Class(doap:CVSRepository))
Declaration(Class(doap:DarcsRepository))
Declaration(Class(doap:GitBranch))
Declaration(Class(doap:GitRepository))
Declaration(Class(doap:HgRepository))
Declaration(Class(doap:Project))
Declaration(Class(doap:Repository))
Declaration(Class(doap:SVNRepository))
Declaration(Class(doap:Specification))
Declaration(Class(doap:Version))
Declaration(Class(rdfs:Resource))
Declaration(Class(<http://xmlns.com/wordnet/1.6/Project>))
Declaration(ObjectProperty(doap:blog))
Declaration(ObjectProperty(doap:developer))
Declaration(ObjectProperty(doap:developer-forum))
Declaration(ObjectProperty(doap:documenter))
Declaration(ObjectProperty(doap:helper))
Declaration(ObjectProperty(doap:homepage))
Declaration(ObjectProperty(doap:implements))
Declaration(ObjectProperty(doap:mailing-list))
Declaration(ObjectProperty(doap:maintainer))
Declaration(ObjectProperty(doap:old-homepage))
Declaration(ObjectProperty(doap:release))
Declaration(ObjectProperty(doap:repository))
Declaration(ObjectProperty(doap:repositoryOf))
Declaration(ObjectProperty(doap:security-contact))
Declaration(ObjectProperty(doap:security-policy))
Declaration(ObjectProperty(doap:service-endpoint))
Declaration(ObjectProperty(doap:support-forum))
Declaration(ObjectProperty(doap:tester))
Declaration(ObjectProperty(doap:translator))
Declaration(ObjectProperty(doap:vendor))
Declaration(ObjectProperty(doap:wiki))
Declaration(DataProperty(doap:anon-root))
Declaration(DataProperty(doap:audience))
Declaration(DataProperty(doap:created))
Declaration(DataProperty(doap:description))
Declaration(DataProperty(doap:language))
Declaration(DataProperty(doap:os))
Declaration(DataProperty(doap:platform))
Declaration(DataProperty(doap:programming-language))
Declaration(DataProperty(doap:revision))
Declaration(DataProperty(doap:shortdesc))
Declaration(NamedIndividual(<http://usefulinc.com/ns/doap#>))
Declaration(NamedIndividual(<mailto:edd@usefulinc.com>))
Declaration(AnnotationProperty(dc:creator))
Declaration(AnnotationProperty(dc:format))
Declaration(AnnotationProperty(dc:rights))
Declaration(AnnotationProperty(doap:browse))
Declaration(AnnotationProperty(doap:bug-database))
Declaration(AnnotationProperty(doap:category))
Declaration(AnnotationProperty(doap:documentation))
Declaration(AnnotationProperty(doap:download-mirror))
Declaration(AnnotationProperty(doap:download-page))
Declaration(AnnotationProperty(doap:file-release))
Declaration(AnnotationProperty(doap:location))
Declaration(AnnotationProperty(doap:module))
Declaration(AnnotationProperty(doap:name))
Declaration(AnnotationProperty(doap:screenshots))
############################
#   Annotation Properties
############################

# Annotation Property: doap:browse (visualiser)

AnnotationAssertion(rdfs:comment doap:browse "Interface web au dépôt."@fr)
AnnotationAssertion(rdfs:comment doap:browse "Interface web del repositorio."@es)
AnnotationAssertion(rdfs:comment doap:browse "Interface web do repositório."@pt)
AnnotationAssertion(rdfs:comment doap:browse "Web browser interface to repository."@en)
AnnotationAssertion(rdfs:comment doap:browse "Web-Browser Interface für das Repository."@de)
AnnotationAssertion(rdfs:comment doap:browse "Webové rozhraní pro prohlížení úložiště."@cs)
AnnotationAssertion(rdfs:isDefinedBy doap:browse <http://usefulinc.com/ns/doap#>)
AnnotationAssertion(rdfs:label doap:browse "browse"@de)
AnnotationAssertion(rdfs:label doap:browse "browse"@en)
AnnotationAssertion(rdfs:label doap:browse "navegar"@es)
AnnotationAssertion(rdfs:label doap:browse "navegar"@pt)
AnnotationAssertion(rdfs:label doap:browse "prohlížeč"@cs)
AnnotationAssertion(rdfs:label doap:browse "visualiser"@fr)
AnnotationPropertyDomain(doap:browse doap:Repository)

# Annotation Property: doap:bug-database (base de datos de bugs)

AnnotationAssertion(rdfs:comment doap:bug-database "Bug tracker for a project."@en)
AnnotationAssertion(rdfs:comment doap:bug-database "Bug tracker para um projeto."@pt)
AnnotationAssertion(rdfs:comment doap:bug-database "Bug tracker para un proyecto."@es)
AnnotationAssertion(rdfs:comment doap:bug-database "Fehlerdatenbank eines Projektes."@de)
AnnotationAssertion(rdfs:comment doap:bug-database "Správa chyb projektu."@cs)
AnnotationAssertion(rdfs:comment doap:bug-database "Suivi des bugs pour un projet."@fr)
AnnotationAssertion(rdfs:isDefinedBy doap:bug-database <http://usefulinc.com/ns/doap#>)
AnnotationAssertion(rdfs:label doap:bug-database "Fehlerdatenbank"@de)
AnnotationAssertion(rdfs:label doap:bug-database "base de dados de bugs"@pt)
AnnotationAssertion(rdfs:label doap:bug-database "base de datos de bugs"@es)
AnnotationAssertion(rdfs:label doap:bug-database "bug database"@en)
AnnotationAssertion(rdfs:label doap:bug-database "databáze chyb"@cs)
AnnotationAssertion(rdfs:label doap:bug-database "suivi des bugs"@fr)
AnnotationPropertyDomain(doap:bug-database doap:Project)

# Annotation Property: doap:category (categoria)

AnnotationAssertion(rdfs:comment doap:category "A category of project."@en)
AnnotationAssertion(rdfs:comment doap:category "Eine Kategorie eines Projektes."@de)
AnnotationAssertion(rdfs:comment doap:category "Kategorie projektu."@cs)
AnnotationAssertion(rdfs:comment doap:category "Uma categoría de projeto."@pt)
AnnotationAssertion(rdfs:comment doap:category "Una categoría de proyecto."@es)
AnnotationAssertion(rdfs:comment doap:category "Une catégorie de projet."@fr)
AnnotationAssertion(rdfs:isDefinedBy doap:category <http://usefulinc.com/ns/doap#>)
AnnotationAssertion(rdfs:label doap:category "Kategorie"@de)
AnnotationAssertion(rdfs:label doap:category "categoria"@pt)
AnnotationAssertion(rdfs:label doap:category "category"@en)
AnnotationAssertion(rdfs:label doap:category "categoría"@es)
AnnotationAssertion(rdfs:label doap:category "catégorie"@fr)
AnnotationAssertion(rdfs:label doap:category "kategorie"@cs)
AnnotationPropertyDomain(doap:category doap:Project)

# Annotation Property: doap:documentation (documentation)

AnnotationAssertion(rdfs:comment doap:documentation "Aide pour l’utilisation de ce projet."@fr)
AnnotationAssertion(rdfs:comment doap:documentation "Documentation of the project."@en)
AnnotationAssertion(rdfs:isDefinedBy doap:documentation <http://usefulinc.com/ns/doap#>)
AnnotationAssertion(rdfs:label doap:documentation "aide"@fr)
AnnotationAssertion(rdfs:label doap:documentation "documentation"@en)
AnnotationPropertyDomain(doap:documentation doap:Project)

# Annotation Property: doap:download-mirror (download mirror)

AnnotationAssertion(rdfs:comment doap:download-mirror "Miroir de la page de téléchargement du programme."@fr)
AnnotationAssertion(rdfs:comment doap:download-mirror "Mirror da página web para fazer download."@pt)
AnnotationAssertion(rdfs:comment doap:download-mirror "Mirror de la página web de descarga."@es)
AnnotationAssertion(rdfs:comment doap:download-mirror "Mirror of software download web page."@en)
AnnotationAssertion(rdfs:comment doap:download-mirror "Spiegel der Seite von die Projekt-Software heruntergeladen werden kann."@de)
AnnotationAssertion(rdfs:comment doap:download-mirror "Zrcadlo stránky pro stažení softwaru."@cs)
AnnotationAssertion(rdfs:isDefinedBy doap:download-mirror <http://usefulinc.com/ns/doap#>)
AnnotationAssertion(rdfs:label doap:download-mirror "Spiegel der Seite zum Herunterladen"@de)
AnnotationAssertion(rdfs:label doap:download-mirror "download mirror"@en)
AnnotationAssertion(rdfs:label doap:download-mirror "miroir pour le téléchargement"@fr)
AnnotationAssertion(rdfs:label doap:download-mirror "mirror de descarga"@es)
AnnotationAssertion(rdfs:label doap:download-mirror "mirror para download"@pt)
AnnotationAssertion(rdfs:label doap:download-mirror "zrcadlo stránky pro stažení"@cs)
AnnotationPropertyDomain(doap:download-mirror doap:Project)

# Annotation Property: doap:download-page (página para download)

AnnotationAssertion(rdfs:comment doap:download-page "Page web à partir de laquelle on peut télécharger le programme."@fr)
AnnotationAssertion(rdfs:comment doap:download-page "Página web da qual o projeto de software pode ser descarregado."@pt)
AnnotationAssertion(rdfs:comment doap:download-page "Página web de la cuál se puede bajar el software."@es)
AnnotationAssertion(rdfs:comment doap:download-page "Web page from which the project software can be downloaded."@en)
AnnotationAssertion(rdfs:comment doap:download-page "Web-Seite von der die Projekt-Software heruntergeladen werden kann."@de)
AnnotationAssertion(rdfs:comment doap:download-page "Webová stránka, na které lze stáhnout projektový software."@cs)
AnnotationAssertion(rdfs:isDefinedBy doap:download-page <http://usefulinc.com/ns/doap#>)
AnnotationAssertion(rdfs:label doap:download-page "Seite zum Herunterladen"@de)
AnnotationAssertion(rdfs:label doap:download-page "download page"@en)
AnnotationAssertion(rdfs:label doap:download-page "page de téléchargement"@fr)
AnnotationAssertion(rdfs:label doap:download-page "página de descarga"@es)
AnnotationAssertion(rdfs:label doap:download-page "página para download"@pt)
AnnotationAssertion(rdfs:label doap:download-page "stránka pro stažení"@cs)
AnnotationPropertyDomain(doap:download-page doap:Project)

# Annotation Property: doap:file-release (publicação do ficheiro)

AnnotationAssertion(rdfs:comment doap:file-release "URI adresa stažení asociované s revizí."@cs)
AnnotationAssertion(rdfs:comment doap:file-release "URI of download associated with this release."@en)
AnnotationAssertion(rdfs:comment doap:file-release "URI para download associado com a publicação."@pt)
AnnotationAssertion(rdfs:isDefinedBy doap:file-release <http://usefulinc.com/ns/doap#>)
AnnotationAssertion(rdfs:label doap:file-release "file-release"@en)
AnnotationAssertion(rdfs:label doap:file-release "publicação do ficheiro"@pt)
AnnotationAssertion(rdfs:label doap:file-release "soubor revize"@cs)
AnnotationPropertyDomain(doap:file-release doap:Version)

# Annotation Property: doap:location (umístění úložiště)

AnnotationAssertion(rdfs:comment doap:location "Emplacement d'un dépôt."@fr)
AnnotationAssertion(rdfs:comment doap:location "Localização de um repositório."@pt)
AnnotationAssertion(rdfs:comment doap:location "Location of a repository."@en)
AnnotationAssertion(rdfs:comment doap:location "Lokation eines Repositorys."@de)
AnnotationAssertion(rdfs:comment doap:location "Umístění úložiště."@cs)
AnnotationAssertion(rdfs:comment doap:location "lugar de un repositorio."@es)
AnnotationAssertion(rdfs:isDefinedBy doap:location <http://usefulinc.com/ns/doap#>)
AnnotationAssertion(rdfs:label doap:location "Repository Lokation"@de)
AnnotationAssertion(rdfs:label doap:location "emplacement du dépôt"@fr)
AnnotationAssertion(rdfs:label doap:location "localização do respositório"@pt)
AnnotationAssertion(rdfs:label doap:location "lugar del respositorio"@es)
AnnotationAssertion(rdfs:label doap:location "repository location"@en)
AnnotationAssertion(rdfs:label doap:location "umístění úložiště"@cs)
AnnotationPropertyDomain(doap:location doap:Repository)

# Annotation Property: doap:module (módulo)

AnnotationAssertion(rdfs:comment doap:module "Jméno modulu v CVS, BitKeeper nebo Arch úložišti."@cs)
AnnotationAssertion(rdfs:comment doap:module "Modul-Name eines Subversion, CVS, BitKeeper oder Arch Repositorys."@de)
AnnotationAssertion(rdfs:comment doap:module "Module name of a Subversion, CVS, BitKeeper or Arch repository."@en)
AnnotationAssertion(rdfs:comment doap:module "Nom du module d'un dépôt Subversion, CVS, BitKeeper ou Arch."@fr)
AnnotationAssertion(rdfs:comment doap:module "Nombre del módulo de un repositorio Subversion, CVS, BitKeeper o Arch."@es)
AnnotationAssertion(rdfs:comment doap:module "Nome do módulo de um repositório Subversion, CVS, BitKeeper ou Arch."@pt)
AnnotationAssertion(rdfs:isDefinedBy doap:module <http://usefulinc.com/ns/doap#>)
AnnotationAssertion(rdfs:label doap:module "Modul"@de)
AnnotationAssertion(rdfs:label doap:module "modul"@cs)
AnnotationAssertion(rdfs:label doap:module "module"@en)
AnnotationAssertion(rdfs:label doap:module "module"@fr)
AnnotationAssertion(rdfs:label doap:module "módulo"@es)
AnnotationAssertion(rdfs:label doap:module "módulo"@pt)
AnnotationPropertyDomain(doap:module <_:genid2147483650>)

# Annotation Property: doap:name (jméno)

AnnotationAssertion(rdfs:comment doap:name "A name of something."@en)
AnnotationAssertion(rdfs:comment doap:name "Der Name von Irgendwas"@de)
AnnotationAssertion(rdfs:comment doap:name "El nombre de algo."@es)
AnnotationAssertion(rdfs:comment doap:name "Jméno něčeho."@cs)
AnnotationAssertion(rdfs:comment doap:name "Le nom de quelque chose."@fr)
AnnotationAssertion(rdfs:comment doap:name "O nome de alguma coisa."@pt)
AnnotationAssertion(rdfs:isDefinedBy doap:name <http://usefulinc.com/ns/doap#>)
AnnotationAssertion(rdfs:label doap:name "Name"@de)
AnnotationAssertion(rdfs:label doap:name "jméno"@cs)
AnnotationAssertion(rdfs:label doap:name "name"@en)
AnnotationAssertion(rdfs:label doap:name "nom"@fr)
AnnotationAssertion(rdfs:label doap:name "nombre"@es)
AnnotationAssertion(rdfs:label doap:name "nome"@pt)
SubAnnotationPropertyOf(doap:name rdfs:label)
AnnotationPropertyRange(doap:name rdfs:Literal)

# Annotation Property: doap:screenshots (captures d'écran)

AnnotationAssertion(rdfs:comment doap:screenshots "Page web avec des captures d'écran du projet."@fr)
AnnotationAssertion(rdfs:comment doap:screenshots "Página web com as capturas de ecrãn do projeto."@pt)
AnnotationAssertion(rdfs:comment doap:screenshots "Página web con capturas de pantalla del proyecto."@es)
AnnotationAssertion(rdfs:comment doap:screenshots "Web page with screenshots of project."@en)
AnnotationAssertion(rdfs:comment doap:screenshots "Web-Seite mit Screenshots eines Projektes."@de)
AnnotationAssertion(rdfs:comment doap:screenshots "Webová stránka projektu se snímky obrazovky."@cs)
AnnotationAssertion(rdfs:isDefinedBy doap:screenshots <http://usefulinc.com/ns/doap#>)
AnnotationAssertion(rdfs:label doap:screenshots "Screenshots"@de)
AnnotationAssertion(rdfs:label doap:screenshots "capturas de ecrãs"@pt)
AnnotationAssertion(rdfs:label doap:screenshots "capturas de pantalla"@es)
AnnotationAssertion(rdfs:label doap:screenshots "captures d'écran"@fr)
AnnotationAssertion(rdfs:label doap:screenshots "screenshots"@en)
AnnotationAssertion(rdfs:label doap:screenshots "snímek obrazovky"@cs)
AnnotationPropertyDomain(doap:screenshots doap:Project)


############################
#   Object Properties
############################

# Object Property: doap:blog (blog)

AnnotationAssertion(rdfs:comment doap:blog "URI de um blog relacionado com um projeto"@pt)
AnnotationAssertion(rdfs:comment doap:blog "URI of a blog related to a project"@en)
AnnotationAssertion(rdfs:isDefinedBy doap:blog <http://usefulinc.com/ns/doap#>)
AnnotationAssertion(rdfs:label doap:blog "blog"@en)
AnnotationAssertion(rdfs:label doap:blog "blog"@pt)
ObjectPropertyDomain(doap:blog doap:Project)
ObjectPropertyRange(doap:blog <http://rdfs.org/sioc/types#Weblog>)
ObjectPropertyRange(doap:blog rdfs:Resource)

# Object Property: doap:developer (desarrollador)

AnnotationAssertion(rdfs:comment doap:developer "Desarrollador de software para el proyecto."@es)
AnnotationAssertion(rdfs:comment doap:developer "Developer of software for the project."@en)
AnnotationAssertion(rdfs:comment doap:developer "Développeur pour le projet."@fr)
AnnotationAssertion(rdfs:comment doap:developer "Programador de software para o projeto."@pt)
AnnotationAssertion(rdfs:comment doap:developer "Software-Entwickler für das Projekt."@de)
AnnotationAssertion(rdfs:comment doap:developer "Vývojář softwaru projektu."@cs)
AnnotationAssertion(rdfs:isDefinedBy doap:developer <http://usefulinc.com/ns/doap#>)
AnnotationAssertion(rdfs:label doap:developer "Entwickler"@de)
AnnotationAssertion(rdfs:label doap:developer "desarrollador"@es)
AnnotationAssertion(rdfs:label doap:developer "developer"@en)
AnnotationAssertion(rdfs:label doap:developer "développeur"@fr)
AnnotationAssertion(rdfs:label doap:developer "programador"@pt)
AnnotationAssertion(rdfs:label doap:developer "vývojář"@cs)
ObjectPropertyDomain(doap:developer doap:Project)
ObjectPropertyRange(doap:developer foaf:Person)

# Object Property: doap:developer-forum (developer forum)

AnnotationAssertion(rdfs:comment doap:developer-forum "A forum or community for developers of this project."@en)
AnnotationAssertion(rdfs:isDefinedBy doap:developer-forum <http://usefulinc.com/ns/doap#>)
AnnotationAssertion(rdfs:label doap:developer-forum "developer forum"@en)
ObjectPropertyDomain(doap:developer-forum doap:Project)
ObjectPropertyRange(doap:developer-forum <http://rdfs.org/sioc/ns#Container>)

# Object Property: doap:documenter (dokumentarista)

AnnotationAssertion(rdfs:comment doap:documenter "Collaborateur à la documentation du projet."@fr)
AnnotationAssertion(rdfs:comment doap:documenter "Contribuidor para a documentação do projeto."@pt)
AnnotationAssertion(rdfs:comment doap:documenter "Contributor of documentation to the project."@en)
AnnotationAssertion(rdfs:comment doap:documenter "Mitarbeiter an der Dokumentation des Projektes."@de)
AnnotationAssertion(rdfs:comment doap:documenter "Proveedor de documentación para el proyecto."@es)
AnnotationAssertion(rdfs:comment doap:documenter "Spoluautor dokumentace projektu."@cs)
AnnotationAssertion(rdfs:isDefinedBy doap:documenter <http://usefulinc.com/ns/doap#>)
AnnotationAssertion(rdfs:label doap:documenter "Dokumentator"@de)
AnnotationAssertion(rdfs:label doap:documenter "documentador"@pt)
AnnotationAssertion(rdfs:label doap:documenter "documenter"@en)
AnnotationAssertion(rdfs:label doap:documenter "dokumentarista"@cs)
AnnotationAssertion(rdfs:label doap:documenter "escritor de ayuda"@es)
AnnotationAssertion(rdfs:label doap:documenter "rédacteur de l'aide"@fr)
ObjectPropertyDomain(doap:documenter doap:Project)
ObjectPropertyRange(doap:documenter foaf:Person)

# Object Property: doap:helper (spoluautor)

AnnotationAssertion(rdfs:comment doap:helper "Ajudante ou colaborador do projeto."@pt)
AnnotationAssertion(rdfs:comment doap:helper "Colaborador del proyecto."@es)
AnnotationAssertion(rdfs:comment doap:helper "Collaborateur au projet."@fr)
AnnotationAssertion(rdfs:comment doap:helper "Project contributor."@en)
AnnotationAssertion(rdfs:comment doap:helper "Projekt-Mitarbeiter."@de)
AnnotationAssertion(rdfs:comment doap:helper "Spoluautor projektu."@cs)
AnnotationAssertion(rdfs:isDefinedBy doap:helper <http://usefulinc.com/ns/doap#>)
AnnotationAssertion(rdfs:label doap:helper "Helfer"@de)
AnnotationAssertion(rdfs:label doap:helper "colaborador"@es)
AnnotationAssertion(rdfs:label doap:helper "colaborador"@pt)
AnnotationAssertion(rdfs:label doap:helper "collaborateur"@fr)
AnnotationAssertion(rdfs:label doap:helper "helper"@en)
AnnotationAssertion(rdfs:label doap:helper "spoluautor"@cs)
ObjectPropertyDomain(doap:helper doap:Project)
ObjectPropertyRange(doap:helper foaf:Person)

# Object Property: doap:homepage (página web)

AnnotationAssertion(rdfs:comment doap:homepage "El URL de la página de un proyecto,
		asociada con exactamente un proyecto."@es)
AnnotationAssertion(rdfs:comment doap:homepage "L'URL de la page web d'un projet,
		associée avec un unique projet."@fr)
AnnotationAssertion(rdfs:comment doap:homepage "O URL da página de um projeto,
		asociada com exactamente um projeto."@pt)
AnnotationAssertion(rdfs:comment doap:homepage "URL adresa domovské stránky projektu asociované s právě jedním projektem."@cs)
AnnotationAssertion(rdfs:comment doap:homepage "URL der Projekt-Homepage,
		verbunden mit genau einem Projekt."@de)
AnnotationAssertion(rdfs:comment doap:homepage "URL of a project's homepage,
		associated with exactly one project."@en)
AnnotationAssertion(rdfs:isDefinedBy doap:homepage <http://usefulinc.com/ns/doap#>)
AnnotationAssertion(rdfs:label doap:homepage "Homepage"@de)
AnnotationAssertion(rdfs:label doap:homepage "domovská stránka"@cs)
AnnotationAssertion(rdfs:label doap:homepage "homepage"@en)
AnnotationAssertion(rdfs:label doap:homepage "page web"@fr)
AnnotationAssertion(rdfs:label doap:homepage "página web"@es)
AnnotationAssertion(rdfs:label doap:homepage "página web"@pt)
SubObjectPropertyOf(doap:homepage foaf:homepage)
InverseFunctionalObjectProperty(doap:homepage)
ObjectPropertyDomain(doap:homepage doap:Project)

# Object Property: doap:implements (Especificações para implementação)

AnnotationAssertion(rdfs:comment doap:implements "A specification that a project implements. Could be a standard, API or legally defined level of conformance."@en)
AnnotationAssertion(rdfs:comment doap:implements "Uma especificação que um projeto implementa. Pode ser uma padrão, API ou um nível de conformidade definida legalmente."@pt)
AnnotationAssertion(rdfs:isDefinedBy doap:implements <http://usefulinc.com/ns/doap#>)
AnnotationAssertion(rdfs:label doap:implements "Especificações para implementação"@pt)
AnnotationAssertion(rdfs:label doap:implements "Implements specification"@en)
ObjectPropertyDomain(doap:implements doap:Project)
ObjectPropertyRange(doap:implements doap:Specification)

# Object Property: doap:mailing-list (liste de diffusion)

AnnotationAssertion(rdfs:comment doap:mailing-list "Domovská stránka nebo e–mailová adresa e–mailové diskuse."@cs)
AnnotationAssertion(rdfs:comment doap:mailing-list "Homepage der Mailing Liste oder E-Mail Adresse."@de)
AnnotationAssertion(rdfs:comment doap:mailing-list "Mailing list home page or email address."@en)
AnnotationAssertion(rdfs:comment doap:mailing-list "Page web de la liste de diffusion, ou adresse de courriel."@fr)
AnnotationAssertion(rdfs:comment doap:mailing-list "Página web da lista de distribuição de e-mail ou dos endereços."@pt)
AnnotationAssertion(rdfs:comment doap:mailing-list "Página web de la lista de correo o dirección de correo."@es)
AnnotationAssertion(rdfs:isDefinedBy doap:mailing-list <http://usefulinc.com/ns/doap#>)
AnnotationAssertion(rdfs:label doap:mailing-list "Mailing Liste"@de)
AnnotationAssertion(rdfs:label doap:mailing-list "e–mailová diskuse"@cs)
AnnotationAssertion(rdfs:label doap:mailing-list "lista de correo"@es)
AnnotationAssertion(rdfs:label doap:mailing-list "lista de distribuição de e-mail"@pt)
AnnotationAssertion(rdfs:label doap:mailing-list "liste de diffusion"@fr)
AnnotationAssertion(rdfs:label doap:mailing-list "mailing list"@en)
ObjectPropertyDomain(doap:mailing-list doap:Project)
ObjectPropertyRange(doap:mailing-list <http://rdfs.org/sioc/types#MailingList>)

# Object Property: doap:maintainer (Projektverantwortlicher)

AnnotationAssertion(rdfs:comment doap:maintainer "Desarrollador principal de un proyecto, un líder de proyecto."@es)
AnnotationAssertion(rdfs:comment doap:maintainer "Développeur principal d'un projet, un meneur du projet."@fr)
AnnotationAssertion(rdfs:comment doap:maintainer "Hauptentwickler eines Projektes, der Projektleiter"@de)
AnnotationAssertion(rdfs:comment doap:maintainer "Maintainer of a project, a project leader."@en)
AnnotationAssertion(rdfs:comment doap:maintainer "Programador principal de um projeto, um líder de projeto."@pt)
AnnotationAssertion(rdfs:comment doap:maintainer "Správce projektu, vedoucí projektu."@cs)
AnnotationAssertion(rdfs:isDefinedBy doap:maintainer <http://usefulinc.com/ns/doap#>)
AnnotationAssertion(rdfs:label doap:maintainer "Projektverantwortlicher"@de)
AnnotationAssertion(rdfs:label doap:maintainer "desarrollador principal"@es)
AnnotationAssertion(rdfs:label doap:maintainer "développeur principal"@fr)
AnnotationAssertion(rdfs:label doap:maintainer "maintainer"@en)
AnnotationAssertion(rdfs:label doap:maintainer "programador principal"@pt)
AnnotationAssertion(rdfs:label doap:maintainer "správce"@cs)
ObjectPropertyDomain(doap:maintainer doap:Project)
ObjectPropertyRange(doap:maintainer foaf:Person)

# Object Property: doap:old-homepage (Alte Homepage)

AnnotationAssertion(rdfs:comment doap:old-homepage "El URL de la antigua página de un proyecto,
		asociada con exactamente un proyecto."@es)
AnnotationAssertion(rdfs:comment doap:old-homepage "L'URL d'une ancienne page web d'un
		projet, associée avec un unique projet."@fr)
AnnotationAssertion(rdfs:comment doap:old-homepage "O URL antigo da página de um projeto,
		associada com exactamente um projeto."@pt)
AnnotationAssertion(rdfs:comment doap:old-homepage "URL adresa předešlé domovské stránky projektu asociované s právě jedním projektem."@cs)
AnnotationAssertion(rdfs:comment doap:old-homepage "URL der letzten Projekt-Homepage,
		verbunden mit genau einem Projekt."@de)
AnnotationAssertion(rdfs:comment doap:old-homepage "URL of a project's past homepage,
		associated with exactly one project."@en)
AnnotationAssertion(rdfs:isDefinedBy doap:old-homepage <http://usefulinc.com/ns/doap#>)
AnnotationAssertion(rdfs:label doap:old-homepage "Alte Homepage"@de)
AnnotationAssertion(rdfs:label doap:old-homepage "ancienne page web"@fr)
AnnotationAssertion(rdfs:label doap:old-homepage "old homepage"@en)
AnnotationAssertion(rdfs:label doap:old-homepage "página web antiga"@pt)
AnnotationAssertion(rdfs:label doap:old-homepage "página web antigua"@es)
AnnotationAssertion(rdfs:label doap:old-homepage "stará domovská stránka"@cs)
SubObjectPropertyOf(doap:old-homepage foaf:homepage)
InverseFunctionalObjectProperty(doap:old-homepage)
ObjectPropertyDomain(doap:old-homepage doap:Project)

# Object Property: doap:release (release)

AnnotationAssertion(rdfs:comment doap:release "A project release."@en)
AnnotationAssertion(rdfs:comment doap:release "A publicação de um projeto."@pt)
AnnotationAssertion(rdfs:comment doap:release "Ein Release (Version) eines Projekts."@de)
AnnotationAssertion(rdfs:comment doap:release "Relase (verze) projektu."@cs)
AnnotationAssertion(rdfs:comment doap:release "Un release (versión) de un proyecto."@es)
AnnotationAssertion(rdfs:comment doap:release "Une release (révision) d'un projet."@fr)
AnnotationAssertion(rdfs:isDefinedBy doap:release <http://usefulinc.com/ns/doap#>)
AnnotationAssertion(rdfs:label doap:release "Release"@de)
AnnotationAssertion(rdfs:label doap:release "publicação"@pt)
AnnotationAssertion(rdfs:label doap:release "release"@cs)
AnnotationAssertion(rdfs:label doap:release "release"@en)
AnnotationAssertion(rdfs:label doap:release "release"@es)
AnnotationAssertion(rdfs:label doap:release "release"@fr)
ObjectPropertyDomain(doap:release doap:Project)
ObjectPropertyRange(doap:release doap:Version)

# Object Property: doap:repository (repositório)

AnnotationAssertion(rdfs:comment doap:repository "Dépôt du code source."@fr)
AnnotationAssertion(rdfs:comment doap:repository "Quellcode-Versionierungssystem."@de)
AnnotationAssertion(rdfs:comment doap:repository "Repositorio del código fuente."@es)
AnnotationAssertion(rdfs:comment doap:repository "Repositório do código fonte."@pt)
AnnotationAssertion(rdfs:comment doap:repository "Source code repository."@en)
AnnotationAssertion(rdfs:comment doap:repository "Úložiště zdrojových kódů."@cs)
AnnotationAssertion(rdfs:isDefinedBy doap:repository <http://usefulinc.com/ns/doap#>)
AnnotationAssertion(rdfs:label doap:repository "Repository"@de)
AnnotationAssertion(rdfs:label doap:repository "dépôt"@fr)
AnnotationAssertion(rdfs:label doap:repository "repositorio"@es)
AnnotationAssertion(rdfs:label doap:repository "repository"@en)
AnnotationAssertion(rdfs:label doap:repository "repositório"@pt)
AnnotationAssertion(rdfs:label doap:repository "úložiště"@cs)
InverseObjectProperties(doap:repository doap:repositoryOf)
ObjectPropertyDomain(doap:repository doap:Project)
ObjectPropertyRange(doap:repository doap:Repository)

# Object Property: doap:repositoryOf (repository of)

AnnotationAssertion(rdfs:comment doap:repositoryOf "The project that uses a repository."@en)
AnnotationAssertion(rdfs:isDefinedBy doap:repositoryOf <http://usefulinc.com/ns/doap#>)
AnnotationAssertion(rdfs:label doap:repositoryOf "repository of"@en)
ObjectPropertyDomain(doap:repositoryOf doap:Repository)
ObjectPropertyRange(doap:repositoryOf doap:Project)

# Object Property: doap:security-contact (security contact)

AnnotationAssertion(rdfs:comment doap:security-contact "The Agent that should be contacted
	if security issues are found with the project."@en)
AnnotationAssertion(rdfs:isDefinedBy doap:security-contact <http://usefulinc.com/ns/doap#>)
AnnotationAssertion(rdfs:label doap:security-contact "security contact"@en)
ObjectPropertyDomain(doap:security-contact doap:Project)
ObjectPropertyRange(doap:security-contact foaf:Agent)

# Object Property: doap:security-policy (security policy)

AnnotationAssertion(rdfs:comment doap:security-policy "URL of the security policy of a project."@en)
AnnotationAssertion(rdfs:isDefinedBy doap:security-policy <http://usefulinc.com/ns/doap#>)
AnnotationAssertion(rdfs:label doap:security-policy "security policy"@en)
SubObjectPropertyOf(doap:security-policy foaf:page)
ObjectPropertyDomain(doap:security-policy doap:Project)

# Object Property: doap:service-endpoint (service endpoint)

AnnotationAssertion(rdfs:comment doap:service-endpoint "The URI of a web service endpoint where software as a service may be accessed"@en)
AnnotationAssertion(rdfs:isDefinedBy doap:service-endpoint <http://usefulinc.com/ns/doap#>)
AnnotationAssertion(rdfs:label doap:service-endpoint "service endpoint"@en)
ObjectPropertyDomain(doap:service-endpoint doap:Project)
ObjectPropertyRange(doap:service-endpoint rdfs:Resource)

# Object Property: doap:support-forum (supporting forum)

AnnotationAssertion(rdfs:comment doap:support-forum "A forum or community that supports this project."@en)
AnnotationAssertion(rdfs:isDefinedBy doap:support-forum <http://usefulinc.com/ns/doap#>)
AnnotationAssertion(rdfs:label doap:support-forum "supporting forum"@en)
ObjectPropertyDomain(doap:support-forum doap:Project)
ObjectPropertyRange(doap:support-forum <http://rdfs.org/sioc/ns#Container>)

# Object Property: doap:tester (tester)

AnnotationAssertion(rdfs:comment doap:tester "A tester or other quality control contributor."@en)
AnnotationAssertion(rdfs:comment doap:tester "Ein Tester oder anderer Mitarbeiter der Qualitätskontrolle."@de)
AnnotationAssertion(rdfs:comment doap:tester "Tester nebo jiný spoluautor kontrolující kvalitu."@cs)
AnnotationAssertion(rdfs:comment doap:tester "Um controlador ou outro contribuidor para o controlo de qualidade."@pt)
AnnotationAssertion(rdfs:comment doap:tester "Un tester u otro proveedor de control de calidad."@es)
AnnotationAssertion(rdfs:comment doap:tester "Un testeur ou un collaborateur au contrôle qualité."@fr)
AnnotationAssertion(rdfs:isDefinedBy doap:tester <http://usefulinc.com/ns/doap#>)
AnnotationAssertion(rdfs:label doap:tester "Tester"@de)
AnnotationAssertion(rdfs:label doap:tester "controlador"@pt)
AnnotationAssertion(rdfs:label doap:tester "tester"@cs)
AnnotationAssertion(rdfs:label doap:tester "tester"@en)
AnnotationAssertion(rdfs:label doap:tester "tester"@es)
AnnotationAssertion(rdfs:label doap:tester "testeur"@fr)
ObjectPropertyDomain(doap:tester doap:Project)
ObjectPropertyRange(doap:tester foaf:Person)

# Object Property: doap:translator (traducteur)

AnnotationAssertion(rdfs:comment doap:translator "Collaborateur à la traduction du projet."@fr)
AnnotationAssertion(rdfs:comment doap:translator "Contribuidor das traduções para o projeto."@pt)
AnnotationAssertion(rdfs:comment doap:translator "Contributor of translations to the project."@en)
AnnotationAssertion(rdfs:comment doap:translator "Mitarbeiter an den Übersetzungen des Projektes."@de)
AnnotationAssertion(rdfs:comment doap:translator "Proveedor de traducciones al proyecto."@es)
AnnotationAssertion(rdfs:comment doap:translator "Spoluautor překladu projektu."@cs)
AnnotationAssertion(rdfs:isDefinedBy doap:translator <http://usefulinc.com/ns/doap#>)
AnnotationAssertion(rdfs:label doap:translator "překladatel"@cs)
AnnotationAssertion(rdfs:label doap:translator "traducteur"@fr)
AnnotationAssertion(rdfs:label doap:translator "traductor"@es)
AnnotationAssertion(rdfs:label doap:translator "tradutor"@pt)
AnnotationAssertion(rdfs:label doap:translator "translator"@en)
AnnotationAssertion(rdfs:label doap:translator "Übersetzer"@de)
ObjectPropertyDomain(doap:translator doap:Project)
ObjectPropertyRange(doap:translator foaf:Person)

# Object Property: doap:vendor (vendor)

AnnotationAssertion(rdfs:comment doap:vendor "Vendor organization: commercial, free or otherwise"@en)
AnnotationAssertion(rdfs:isDefinedBy doap:vendor <http://usefulinc.com/ns/doap#>)
AnnotationAssertion(rdfs:label doap:vendor "vendor"@en)
ObjectPropertyDomain(doap:vendor doap:Project)
ObjectPropertyRange(doap:vendor foaf:Organization)

# Object Property: doap:wiki (Wiki)

AnnotationAssertion(rdfs:comment doap:wiki "L'URL du Wiki pour la discussion collaborative sur le projet."@fr)
AnnotationAssertion(rdfs:comment doap:wiki "URL adresa wiki projektu pro společné diskuse."@cs)
AnnotationAssertion(rdfs:comment doap:wiki "URL da Wiki para discussão em grupo do projeto."@pt)
AnnotationAssertion(rdfs:comment doap:wiki "URL del Wiki para discusión colaborativa del proyecto."@es)
AnnotationAssertion(rdfs:comment doap:wiki "URL of Wiki for collaborative discussion of project."@en)
AnnotationAssertion(rdfs:comment doap:wiki "Wiki-URL für die kollaborative Dikussion eines Projektes."@de)
AnnotationAssertion(rdfs:isDefinedBy doap:wiki <http://usefulinc.com/ns/doap#>)
AnnotationAssertion(rdfs:label doap:wiki "Wiki"@de)
AnnotationAssertion(rdfs:label doap:wiki "wiki"@cs)
AnnotationAssertion(rdfs:label doap:wiki "wiki"@en)
AnnotationAssertion(rdfs:label doap:wiki "wiki"@es)
AnnotationAssertion(rdfs:label doap:wiki "wiki"@fr)
AnnotationAssertion(rdfs:label doap:wiki "wiki"@pt)
ObjectPropertyDomain(doap:wiki doap:Project)
ObjectPropertyRange(doap:wiki <http://rdfs.org/sioc/types#Wiki>)


############################
#   Data Properties
############################

# Data Property: doap:anon-root (racine anonyme)

AnnotationAssertion(rdfs:comment doap:anon-root "Dépôt pour accès anonyme."@fr)
AnnotationAssertion(rdfs:comment doap:anon-root "Repositorio para acceso anónimo."@es)
AnnotationAssertion(rdfs:comment doap:anon-root "Repository for anonymous access."@en)
AnnotationAssertion(rdfs:comment doap:anon-root "Repository für anonymen Zugriff"@de)
AnnotationAssertion(rdfs:comment doap:anon-root "Repositório para acesso anónimo."@pt)
AnnotationAssertion(rdfs:comment doap:anon-root "Úložiště pro anonymní přístup."@cs)
AnnotationAssertion(rdfs:isDefinedBy doap:anon-root <http://usefulinc.com/ns/doap#>)
AnnotationAssertion(rdfs:label doap:anon-root "Anonymes Root"@de)
AnnotationAssertion(rdfs:label doap:anon-root "anonymní kořen"@cs)
AnnotationAssertion(rdfs:label doap:anon-root "anonymous root"@en)
AnnotationAssertion(rdfs:label doap:anon-root "racine anonyme"@fr)
AnnotationAssertion(rdfs:label doap:anon-root "raíz anónima"@es)
AnnotationAssertion(rdfs:label doap:anon-root "raíz anónima"@pt)
DataPropertyDomain(doap:anon-root doap:Repository)
DataPropertyRange(doap:anon-root rdfs:Literal)

# Data Property: doap:audience (audience)

AnnotationAssertion(rdfs:comment doap:audience "Description of target user base"@en)
AnnotationAssertion(rdfs:comment doap:audience "Descrição do utilizador base alvo"@pt)
AnnotationAssertion(rdfs:isDefinedBy doap:audience <http://usefulinc.com/ns/doap#>)
AnnotationAssertion(rdfs:label doap:audience "audience"@en)
AnnotationAssertion(rdfs:label doap:audience "audiência"@pt)
DataPropertyDomain(doap:audience doap:Project)
DataPropertyRange(doap:audience rdfs:Literal)

# Data Property: doap:created (vytvořeno)

AnnotationAssertion(rdfs:comment doap:created "Data em que algo foi criado, no formato AAAA-MM-DD. e.g. 2004-04-05"@pt)
AnnotationAssertion(rdfs:comment doap:created "Date when something was created, in YYYY-MM-DD form. e.g. 2004-04-05"@en)
AnnotationAssertion(rdfs:comment doap:created "Date à laquelle a été créé quelque chose, au format AAAA-MM-JJ (par ex. 2004-04-05)"@fr)
AnnotationAssertion(rdfs:comment doap:created "Datum, kdy bylo něco vytvořeno ve formátu RRRR-MM-DD, např. 2004-04-05"@cs)
AnnotationAssertion(rdfs:comment doap:created "Erstellungsdatum von Irgendwas, angegeben im YYYY-MM-DD Format, z.B. 2004-04-05."@de)
AnnotationAssertion(rdfs:comment doap:created "Fecha en la que algo fue creado, en formato AAAA-MM-DD. e.g. 2004-04-05"@es)
AnnotationAssertion(rdfs:isDefinedBy doap:created <http://usefulinc.com/ns/doap#>)
AnnotationAssertion(rdfs:label doap:created "creado"@es)
AnnotationAssertion(rdfs:label doap:created "created"@en)
AnnotationAssertion(rdfs:label doap:created "criado"@pt)
AnnotationAssertion(rdfs:label doap:created "créé"@fr)
AnnotationAssertion(rdfs:label doap:created "erstellt"@de)
AnnotationAssertion(rdfs:label doap:created "vytvořeno"@cs)
DataPropertyRange(doap:created rdfs:Literal)

# Data Property: doap:description (description)

AnnotationAssertion(rdfs:comment doap:description "Beschreibung eines Projekts als einfacher Text mit der Länge von 2 bis 4 Sätzen."@de)
AnnotationAssertion(rdfs:comment doap:description "Descripción en texto plano de un proyecto, de 2 a 4 enunciados de longitud."@es)
AnnotationAssertion(rdfs:comment doap:description "Descrição de um projeto em texto apenas, com 2 a 4 frases de comprimento."@pt)
AnnotationAssertion(rdfs:comment doap:description "Plain text description of a project, of 2-4 sentences in length."@en)
AnnotationAssertion(rdfs:comment doap:description "Texte descriptif d'un projet, long de 2 à 4 phrases."@fr)
AnnotationAssertion(rdfs:comment doap:description "Čistě textový, 2 až 4 věty dlouhý popis projektu."@cs)
AnnotationAssertion(rdfs:isDefinedBy doap:description <http://usefulinc.com/ns/doap#>)
AnnotationAssertion(rdfs:label doap:description "Beschreibung"@de)
AnnotationAssertion(rdfs:label doap:description "descripción"@es)
AnnotationAssertion(rdfs:label doap:description "description"@en)
AnnotationAssertion(rdfs:label doap:description "description"@fr)
AnnotationAssertion(rdfs:label doap:description "descrição"@pt)
AnnotationAssertion(rdfs:label doap:description "popis"@cs)
DataPropertyRange(doap:description rdfs:Literal)

# Data Property: doap:language (language)

AnnotationAssertion(rdfs:comment doap:language "BCP47 language code a project has been translated into"@en)
AnnotationAssertion(rdfs:comment doap:language "Código de idioma BCP47 do projeto para o qual foi traduzido"@pt)
AnnotationAssertion(rdfs:isDefinedBy doap:language <http://usefulinc.com/ns/doap#>)
AnnotationAssertion(rdfs:label doap:language "idioma"@pt)
AnnotationAssertion(rdfs:label doap:language "language"@en)
DataPropertyDomain(doap:language doap:Project)
DataPropertyRange(doap:language rdfs:Literal)

# Data Property: doap:os (sistema operativo)

AnnotationAssertion(rdfs:comment doap:os "Betriebssystem auf dem das Projekt eingesetzt werden kann. Diese Eigenschaft kann ausgelassen werden, wenn das Projekt nicht BS-spezifisch ist."@de)
AnnotationAssertion(rdfs:comment doap:os "Operating system that a project is limited to.  Omit this property if the project is not OS-specific."@en)
AnnotationAssertion(rdfs:comment doap:os "Operační systém, na jehož použití je projekt limitován. Vynechejte tuto vlastnost, pokud je projekt nezávislý na operačním systému."@cs)
AnnotationAssertion(rdfs:comment doap:os "Sistema operativo a que o projeto está limitado. Omita esta propriedade se o projeto não é condicionado pelo SO usado."@en)
AnnotationAssertion(rdfs:comment doap:os "Sistema opertivo al cuál está limitado el proyecto.  Omita esta propiedad si el proyecto no es específico
		de un sistema opertaivo en particular."@es)
AnnotationAssertion(rdfs:comment doap:os "Système d'exploitation auquel est limité le projet. Omettez cette propriété si le
		projet n'est pas limité à un système d'exploitation."@fr)
AnnotationAssertion(rdfs:isDefinedBy doap:os <http://usefulinc.com/ns/doap#>)
AnnotationAssertion(rdfs:label doap:os "Betriebssystem"@de)
AnnotationAssertion(rdfs:label doap:os "operating system"@en)
AnnotationAssertion(rdfs:label doap:os "operační systém"@cs)
AnnotationAssertion(rdfs:label doap:os "sistema operativo"@es)
AnnotationAssertion(rdfs:label doap:os "sistema operativo"@pt)
AnnotationAssertion(rdfs:label doap:os "système d'exploitation"@fr)
DataPropertyDomain(doap:os doap:Project)
DataPropertyDomain(doap:os doap:Version)
DataPropertyRange(doap:os rdfs:Literal)

# Data Property: doap:platform (plataforma)

AnnotationAssertion(rdfs:comment doap:platform "Indicador da plataforma do software (não específico a nenhum SO), ex.: Java, Firefox, ECMA CLR"@pt)
AnnotationAssertion(rdfs:comment doap:platform "Indicator of software platform (non-OS specific), e.g. Java, Firefox, ECMA CLR"@en)
AnnotationAssertion(rdfs:isDefinedBy doap:platform <http://usefulinc.com/ns/doap#>)
AnnotationAssertion(rdfs:label doap:platform "plataforma"@pt)
AnnotationAssertion(rdfs:label doap:platform "platform"@en)
DataPropertyDomain(doap:platform doap:Project)
DataPropertyDomain(doap:platform doap:Version)
DataPropertyRange(doap:platform rdfs:Literal)

# Data Property: doap:programming-language (linguagem de programação)

AnnotationAssertion(rdfs:comment doap:programming-language "Langage de programmation avec lequel un projet est implémenté,
		ou avec lequel il est prévu de l'utiliser."@fr)
AnnotationAssertion(rdfs:comment doap:programming-language "Lenguaje de programación en el que un proyecto es implementado o con el cuál pretende usarse."@es)
AnnotationAssertion(rdfs:comment doap:programming-language "Linguagem de programação que o projeto usa ou é para ser utilizada."@pt)
AnnotationAssertion(rdfs:comment doap:programming-language "Programmiersprache in der ein Projekt implementiert ist oder intendiert wird zu benutzen."@de)
AnnotationAssertion(rdfs:comment doap:programming-language "Programming language a project is implemented in or intended for use with."@en)
AnnotationAssertion(rdfs:comment doap:programming-language "Programovací jazyk, ve kterém je projekt implementován nebo pro který je zamýšlen k použití."@cs)
AnnotationAssertion(rdfs:isDefinedBy doap:programming-language <http://usefulinc.com/ns/doap#>)
AnnotationAssertion(rdfs:label doap:programming-language "Programmiersprache"@de)
AnnotationAssertion(rdfs:label doap:programming-language "langage de programmation"@fr)
AnnotationAssertion(rdfs:label doap:programming-language "lenguaje de programación"@es)
AnnotationAssertion(rdfs:label doap:programming-language "linguagem de programação"@pt)
AnnotationAssertion(rdfs:label doap:programming-language "programming language"@en)
AnnotationAssertion(rdfs:label doap:programming-language "programovací jazyk"@cs)
DataPropertyDomain(doap:programming-language doap:Project)
DataPropertyRange(doap:programming-language rdfs:Literal)

# Data Property: doap:revision (Version)

AnnotationAssertion(rdfs:comment doap:revision "Identifiant de révision d'une release du programme."@fr)
AnnotationAssertion(rdfs:comment doap:revision "Identificador do lançamento da revisão do software."@pt)
AnnotationAssertion(rdfs:comment doap:revision "Identifikátor zpřístupněné revize softwaru."@cs)
AnnotationAssertion(rdfs:comment doap:revision "Indentificador de la versión de un release de software."@es)
AnnotationAssertion(rdfs:comment doap:revision "Revision identifier of a software release."@en)
AnnotationAssertion(rdfs:comment doap:revision "Versionsidentifikator eines Software-Releases."@de)
AnnotationAssertion(rdfs:isDefinedBy doap:revision <http://usefulinc.com/ns/doap#>)
AnnotationAssertion(rdfs:label doap:revision "Version"@de)
AnnotationAssertion(rdfs:label doap:revision "revision"@en)
AnnotationAssertion(rdfs:label doap:revision "revisão"@pt)
AnnotationAssertion(rdfs:label doap:revision "révision"@fr)
AnnotationAssertion(rdfs:label doap:revision "versión"@es)
AnnotationAssertion(rdfs:label doap:revision "verze"@cs)
DataPropertyDomain(doap:revision doap:Version)
DataPropertyRange(doap:revision rdfs:Literal)

# Data Property: doap:shortdesc (description courte)

AnnotationAssertion(rdfs:comment doap:shortdesc "Descripción corta (8 o 9 palabras) en texto plano de un proyecto."@es)
AnnotationAssertion(rdfs:comment doap:shortdesc "Descrição curta (com 8 ou 9 palavras) de um projeto em texto apenas."@pt)
AnnotationAssertion(rdfs:comment doap:shortdesc "Krátký (8 nebo 9 slov) čistě textový popis projektu."@cs)
AnnotationAssertion(rdfs:comment doap:shortdesc "Kurzbeschreibung (8 oder 9 Wörter) eines Projekts als einfacher Text."@de)
AnnotationAssertion(rdfs:comment doap:shortdesc "Short (8 or 9 words) plain text description of a project."@en)
AnnotationAssertion(rdfs:comment doap:shortdesc "Texte descriptif concis (8 ou 9 mots) d'un projet."@fr)
AnnotationAssertion(rdfs:isDefinedBy doap:shortdesc <http://usefulinc.com/ns/doap#>)
AnnotationAssertion(rdfs:label doap:shortdesc "Kurzbeschreibung"@de)
AnnotationAssertion(rdfs:label doap:shortdesc "descripción corta"@es)
AnnotationAssertion(rdfs:label doap:shortdesc "description courte"@fr)
AnnotationAssertion(rdfs:label doap:shortdesc "descrição curta"@pt)
AnnotationAssertion(rdfs:label doap:shortdesc "krátký popis"@cs)
AnnotationAssertion(rdfs:label doap:shortdesc "short description"@en)
DataPropertyRange(doap:shortdesc rdfs:Literal)



############################
#   Classes
############################

# Class: doap:ArchRepository (Repositório GNU Arch)

AnnotationAssertion(rdfs:comment doap:ArchRepository "Dépôt GNU Arch du code source."@fr)
AnnotationAssertion(rdfs:comment doap:ArchRepository "GNU Arch Quellcode-Versionierungssystem."@de)
AnnotationAssertion(rdfs:comment doap:ArchRepository "GNU Arch source code repository."@en)
AnnotationAssertion(rdfs:comment doap:ArchRepository "Repositorio GNU Arch del código fuente."@es)
AnnotationAssertion(rdfs:comment doap:ArchRepository "Repositório GNU Arch do código fonte."@pt)
AnnotationAssertion(rdfs:comment doap:ArchRepository "Úložiště zdrojových kódů GNU Arch."@cs)
AnnotationAssertion(rdfs:isDefinedBy doap:ArchRepository <http://usefulinc.com/ns/doap#>)
AnnotationAssertion(rdfs:label doap:ArchRepository "Dépôt GNU Arch"@fr)
AnnotationAssertion(rdfs:label doap:ArchRepository "GNU Arch repository"@de)
AnnotationAssertion(rdfs:label doap:ArchRepository "GNU Arch repository"@en)
AnnotationAssertion(rdfs:label doap:ArchRepository "Repositorio GNU Arch"@es)
AnnotationAssertion(rdfs:label doap:ArchRepository "Repositório GNU Arch"@pt)
AnnotationAssertion(rdfs:label doap:ArchRepository "Úložiště GNU Arch"@cs)
SubClassOf(doap:ArchRepository doap:Repository)

# Class: doap:BKRepository (BitKeeper Repository)

AnnotationAssertion(rdfs:comment doap:BKRepository "BitKeeper Quellcode-Versionierungssystem."@de)
AnnotationAssertion(rdfs:comment doap:BKRepository "BitKeeper source code repository."@en)
AnnotationAssertion(rdfs:comment doap:BKRepository "Dépôt BitKeeper du code source."@fr)
AnnotationAssertion(rdfs:comment doap:BKRepository "Repositorio BitKeeper del código fuente."@es)
AnnotationAssertion(rdfs:comment doap:BKRepository "Repositório BitKeeper do código fonte."@pt)
AnnotationAssertion(rdfs:comment doap:BKRepository "Úložiště zdrojových kódů BitKeeper."@cs)
AnnotationAssertion(rdfs:isDefinedBy doap:BKRepository <http://usefulinc.com/ns/doap#>)
AnnotationAssertion(rdfs:label doap:BKRepository "BitKeeper Repository"@de)
AnnotationAssertion(rdfs:label doap:BKRepository "BitKeeper Repository"@en)
AnnotationAssertion(rdfs:label doap:BKRepository "Dépôt BitKeeper"@fr)
AnnotationAssertion(rdfs:label doap:BKRepository "Repositorio BitKeeper"@es)
AnnotationAssertion(rdfs:label doap:BKRepository "Repositório Bitkeeper"@pt)
AnnotationAssertion(rdfs:label doap:BKRepository "Úložiště BitKeeper"@cs)
SubClassOf(doap:BKRepository doap:Repository)

# Class: doap:BazaarBranch (Ramificação Bazaar)

AnnotationAssertion(rdfs:comment doap:BazaarBranch "Bazaar source code branch."@en)
AnnotationAssertion(rdfs:comment doap:BazaarBranch "Código fonte da ramificação Bazaar."@pt)
AnnotationAssertion(rdfs:isDefinedBy doap:BazaarBranch <http://usefulinc.com/ns/doap#>)
AnnotationAssertion(rdfs:label doap:BazaarBranch "Bazaar Branch"@en)
AnnotationAssertion(rdfs:label doap:BazaarBranch "Ramificação Bazaar"@pt)
SubClassOf(doap:BazaarBranch doap:Repository)

# Class: doap:CVSRepository (Dépôt CVS)

AnnotationAssertion(rdfs:comment doap:CVSRepository "CVS Quellcode-Versionierungssystem."@de)
AnnotationAssertion(rdfs:comment doap:CVSRepository "CVS source code repository."@en)
AnnotationAssertion(rdfs:comment doap:CVSRepository "Dépôt CVS du code source."@fr)
AnnotationAssertion(rdfs:comment doap:CVSRepository "Repositorio CVS del código fuente."@es)
AnnotationAssertion(rdfs:comment doap:CVSRepository "Repositório CVS do código fonte."@pt)
AnnotationAssertion(rdfs:comment doap:CVSRepository "Úložiště zdrojových kódů CVS."@cs)
AnnotationAssertion(rdfs:isDefinedBy doap:CVSRepository <http://usefulinc.com/ns/doap#>)
AnnotationAssertion(rdfs:label doap:CVSRepository "CVS Repository"@de)
AnnotationAssertion(rdfs:label doap:CVSRepository "CVS Repository"@en)
AnnotationAssertion(rdfs:label doap:CVSRepository "Dépôt CVS"@fr)
AnnotationAssertion(rdfs:label doap:CVSRepository "Repositorio CVS"@es)
AnnotationAssertion(rdfs:label doap:CVSRepository "Repositório CVS"@pt)
AnnotationAssertion(rdfs:label doap:CVSRepository "Úložiště CVS"@cs)
SubClassOf(doap:CVSRepository doap:Repository)

# Class: doap:DarcsRepository (darcs Repository)

AnnotationAssertion(rdfs:comment doap:DarcsRepository "Dépôt darcs du code source."@fr)
AnnotationAssertion(rdfs:comment doap:DarcsRepository "Repositorio darcs del código fuente."@es)
AnnotationAssertion(rdfs:comment doap:DarcsRepository "Repositório darcs do código fonte."@pt)
AnnotationAssertion(rdfs:comment doap:DarcsRepository "darcs source code repository."@en)
AnnotationAssertion(rdfs:isDefinedBy doap:DarcsRepository <http://usefulinc.com/ns/doap#>)
AnnotationAssertion(rdfs:label doap:DarcsRepository "Dépôt darcs"@fr)
AnnotationAssertion(rdfs:label doap:DarcsRepository "Repositorio darcs"@es)
AnnotationAssertion(rdfs:label doap:DarcsRepository "Repositório darcs"@pt)
AnnotationAssertion(rdfs:label doap:DarcsRepository "darcs Repository"@en)
SubClassOf(doap:DarcsRepository doap:Repository)

# Class: doap:GitBranch (Ramificação Git)

AnnotationAssertion(rdfs:comment doap:GitBranch "Código fonte da ramificação Git."@pt)
AnnotationAssertion(rdfs:comment doap:GitBranch "Git source code branch."@en)
AnnotationAssertion(rdfs:isDefinedBy doap:GitBranch <http://usefulinc.com/ns/doap#>)
AnnotationAssertion(rdfs:label doap:GitBranch "Git Branch"@en)
AnnotationAssertion(rdfs:label doap:GitBranch "Ramificação Git"@pt)
SubClassOf(doap:GitBranch doap:Repository)

# Class: doap:GitRepository (Repositorio Git)

AnnotationAssertion(rdfs:comment doap:GitRepository "Dépôt Git du code source."@fr)
AnnotationAssertion(rdfs:comment doap:GitRepository "Git Quellcode-Versionierungssystem."@de)
AnnotationAssertion(rdfs:comment doap:GitRepository "Git source code repository."@en)
AnnotationAssertion(rdfs:comment doap:GitRepository "Repositorio Git del código fuente."@es)
AnnotationAssertion(rdfs:comment doap:GitRepository "Repositório Git do código fonte."@pt)
AnnotationAssertion(rdfs:comment doap:GitRepository "Úložiště zdrojových kódů Git."@cs)
AnnotationAssertion(rdfs:isDefinedBy doap:GitRepository <http://usefulinc.com/ns/doap#>)
AnnotationAssertion(rdfs:label doap:GitRepository "Dépôt Git"@fr)
AnnotationAssertion(rdfs:label doap:GitRepository "Git Repository"@de)
AnnotationAssertion(rdfs:label doap:GitRepository "Git Repository"@en)
AnnotationAssertion(rdfs:label doap:GitRepository "Repositorio Git"@es)
AnnotationAssertion(rdfs:label doap:GitRepository "Repositório Git"@pt)
AnnotationAssertion(rdfs:label doap:GitRepository "Úložiště Git"@cs)
SubClassOf(doap:GitRepository doap:Repository)

# Class: doap:HgRepository (Mercurial Repository)

AnnotationAssertion(rdfs:comment doap:HgRepository "Mercurial source code repository."@en)
AnnotationAssertion(rdfs:comment doap:HgRepository "Repositório Mercurial do código fonte."@pt)
AnnotationAssertion(rdfs:isDefinedBy doap:HgRepository <http://usefulinc.com/ns/doap#>)
AnnotationAssertion(rdfs:label doap:HgRepository "Mercurial Repository"@en)
AnnotationAssertion(rdfs:label doap:HgRepository "Repositório Mercurial"@pt)
SubClassOf(doap:HgRepository doap:Repository)

# Class: doap:Project (Project)

AnnotationAssertion(rdfs:comment doap:Project "A project."@en)
AnnotationAssertion(rdfs:comment doap:Project "Ein Projekt."@de)
AnnotationAssertion(rdfs:comment doap:Project "Projekt."@cs)
AnnotationAssertion(rdfs:comment doap:Project "Projeto."@pt)
AnnotationAssertion(rdfs:comment doap:Project "Un projet."@fr)
AnnotationAssertion(rdfs:comment doap:Project "Un proyecto."@es)
AnnotationAssertion(rdfs:isDefinedBy doap:Project <http://usefulinc.com/ns/doap#>)
AnnotationAssertion(rdfs:label doap:Project "Project"@en)
AnnotationAssertion(rdfs:label doap:Project "Projekt"@cs)
AnnotationAssertion(rdfs:label doap:Project "Projekt"@de)
AnnotationAssertion(rdfs:label doap:Project "Projet"@fr)
AnnotationAssertion(rdfs:label doap:Project "Projeto"@pt)
AnnotationAssertion(rdfs:label doap:Project "Proyecto"@es)
SubClassOf(doap:Project foaf:Project)
SubClassOf(doap:Project <http://xmlns.com/wordnet/1.6/Project>)

# Class: doap:Repository (Repositório)

AnnotationAssertion(rdfs:comment doap:Repository "Dépôt du code source."@fr)
AnnotationAssertion(rdfs:comment doap:Repository "Quellcode-Versionierungssystem."@de)
AnnotationAssertion(rdfs:comment doap:Repository "Repositorio del código fuente."@es)
AnnotationAssertion(rdfs:comment doap:Repository "Repositório do código fonte."@pt)
AnnotationAssertion(rdfs:comment doap:Repository "Source code repository."@en)
AnnotationAssertion(rdfs:comment doap:Repository "Úložiště zdrojových kódů."@cs)
AnnotationAssertion(rdfs:isDefinedBy doap:Repository <http://usefulinc.com/ns/doap#>)
AnnotationAssertion(rdfs:label doap:Repository "Dépôt"@fr)
AnnotationAssertion(rdfs:label doap:Repository "Repositorio"@es)
AnnotationAssertion(rdfs:label doap:Repository "Repository"@de)
AnnotationAssertion(rdfs:label doap:Repository "Repository"@en)
AnnotationAssertion(rdfs:label doap:Repository "Repositório"@pt)
AnnotationAssertion(rdfs:label doap:Repository "Úložiště"@cs)

# Class: doap:SVNRepository (Dépôt Subversion)

AnnotationAssertion(rdfs:comment doap:SVNRepository "Dépôt Subversion du code source."@fr)
AnnotationAssertion(rdfs:comment doap:SVNRepository "Repositorio Subversion del código fuente."@es)
AnnotationAssertion(rdfs:comment doap:SVNRepository "Repositório Subversion do código fonte."@pt)
AnnotationAssertion(rdfs:comment doap:SVNRepository "Subversion Quellcode-Versionierungssystem."@de)
AnnotationAssertion(rdfs:comment doap:SVNRepository "Subversion source code repository."@en)
AnnotationAssertion(rdfs:comment doap:SVNRepository "Úložiště zdrojových kódů Subversion."@cs)
AnnotationAssertion(rdfs:isDefinedBy doap:SVNRepository <http://usefulinc.com/ns/doap#>)
AnnotationAssertion(rdfs:label doap:SVNRepository "Dépôt Subversion"@fr)
AnnotationAssertion(rdfs:label doap:SVNRepository "Repositorio Subversion"@es)
AnnotationAssertion(rdfs:label doap:SVNRepository "Repositório Subversion"@pt)
AnnotationAssertion(rdfs:label doap:SVNRepository "Subversion Repository"@de)
AnnotationAssertion(rdfs:label doap:SVNRepository "Subversion Repository"@en)
AnnotationAssertion(rdfs:label doap:SVNRepository "Úložiště Subversion"@cs)
SubClassOf(doap:SVNRepository doap:Repository)

# Class: doap:Specification (Specification)

AnnotationAssertion(rdfs:comment doap:Specification "A especificação de aspetos, técnicas ou outros do sistema."@pt)
AnnotationAssertion(rdfs:comment doap:Specification "A specification of a system's aspects, technical or otherwise."@en)
AnnotationAssertion(rdfs:isDefinedBy doap:Specification <http://usefulinc.com/ns/doap#>)
AnnotationAssertion(rdfs:label doap:Specification "Especificação"@pt)
AnnotationAssertion(rdfs:label doap:Specification "Specification"@en)
SubClassOf(doap:Specification rdfs:Resource)

# Class: doap:Version (Version)

AnnotationAssertion(rdfs:comment doap:Version "Détails sur une version d'une release d'un projet."@fr)
AnnotationAssertion(rdfs:comment doap:Version "Informace o uvolněné verzi projektu."@cs)
AnnotationAssertion(rdfs:comment doap:Version "Información sobre la versión de un release del proyecto."@es)
AnnotationAssertion(rdfs:comment doap:Version "Informação sobre a versão do projeto lançado."@pt)
AnnotationAssertion(rdfs:comment doap:Version "Version information of a project release."@en)
AnnotationAssertion(rdfs:comment doap:Version "Versionsinformation eines Projekt Releases."@de)
AnnotationAssertion(rdfs:isDefinedBy doap:Version <http://usefulinc.com/ns/doap#>)
AnnotationAssertion(rdfs:label doap:Version "Version"@de)
AnnotationAssertion(rdfs:label doap:Version "Version"@en)
AnnotationAssertion(rdfs:label doap:Version "Version"@fr)
AnnotationAssertion(rdfs:label doap:Version "Versión"@es)
AnnotationAssertion(rdfs:label doap:Version "Versão"@pt)
AnnotationAssertion(rdfs:label doap:Version "Verze"@cs)


############################
#   Named Individuals
############################

# Individual: doap: (doap:)

ObjectPropertyAssertion(foaf:maker <http://usefulinc.com/ns/doap#> _:genid2147483649)


ClassAssertion(foaf:Person _:genid2147483649)
ObjectPropertyAssertion(foaf:mbox _:genid2147483649 <mailto:edd@usefulinc.com>)
DataPropertyAssertion(foaf:name _:genid2147483649 "Edd Wilder-James")
AnnotationAssertion(rdfs:comment doap:license "Die URI einer RDF-Beschreibung einer Lizenz unter der die Software herausgegeben wird. z.B. eine SPDX Referenz"@de)
AnnotationAssertion(rdfs:comment doap:license "El URI de una descripción RDF de la licencia bajo la cuál se distribuye el software."@es)
AnnotationAssertion(rdfs:comment doap:license "L'URI d'une description RDF de la licence sous laquelle le programme est distribué."@fr)
AnnotationAssertion(rdfs:comment doap:license "O URI de uma descrição RDF da licença do software sob a qual é distribuída. Ex.: referência SPDX"@pt)
AnnotationAssertion(rdfs:comment doap:license "The URI of an RDF description of the license the software is distributed under. E.g. a SPDX reference"@en)
AnnotationAssertion(rdfs:comment doap:license "URI adresa RDF popisu licence, pod kterou je software distribuován."@cs)
AnnotationAssertion(rdfs:isDefinedBy doap:license <http://usefulinc.com/ns/doap#>)
AnnotationAssertion(rdfs:label doap:license "Lizenz"@de)
AnnotationAssertion(rdfs:label doap:license "licence"@cs)
AnnotationAssertion(rdfs:label doap:license "licence"@fr)
AnnotationAssertion(rdfs:label doap:license "licencia"@es)
AnnotationAssertion(rdfs:label doap:license "license"@en)
AnnotationAssertion(rdfs:label doap:license "licença"@pt)
)
